agda demo progress + further isabelle cleanup

isabelle/a2.thy
@@ -34,57 +34,43 @@ if @{term x} does not appear in @{term ls} and returns @{term "Some n"}
  The @{term nat} value is offset by 1 because we start from
 @{term "Some 0"} when @{term x} appears once in @{term ls}.
 \<close>
+
 primrec m_count :: "'a list \<Rightarrow> ('a, nat) map" where
-  "m_count [] = Map.empty" (* K NONE *)
-| "m_count (a#as) =
+  "m_count [] = Map.empty"
+|  "m_count (a#as) =
     (case (m_count as) a of
-       None \<Rightarrow> (m_count as)(a\<mapsto>0)
-     | Some n \<Rightarrow> (m_count as)(a\<mapsto>Suc n))"
+   None \<Rightarrow> (m_count as)(a\<mapsto>0)
+| Some n \<Rightarrow> (m_count as)(a\<mapsto>Suc n))"
+print_theorems
 
 value "m_count [0::nat,0,0,2,1,3,2] 0"
-value "count_list [0::nat,0,0,2,1,3,2] 0"
+
 
 text \<open>
 1-(a) State the correspondence between Isabelle's @{term count_list} and
  @{term m_count} as logical equality and prove it.
 \<close>
+
 lemma m_count_corres0:
   "(m_count ls x = None \<longleftrightarrow> count_list ls x = 0)"
   apply(induct ls)
-   apply(simp)
-  apply(simp split: option.splits)
-  done
+  by (auto split: option.splits)
 
 lemma m_count_corres2: "(m_count ls x = None \<longleftrightarrow> count_list ls x = 0) \<and>
                        (m_count ls x = Some n \<longleftrightarrow> count_list ls x = n+1)"
-  apply(rule conjI)
-   apply(simp add: m_count_corres0)
+
   apply(induct ls arbitrary: n)
-   apply(simp)
-  apply(drule_tac allI)
-  apply(rename_tac m)
-  apply(simp)
-  apply(rule conjI)
-   apply(case_tac "m_count ls x")
-    apply(drule_tac x=n in allE)
-     apply(simp)
-    apply(simp)
-    apply(simp add: m_count_corres0)
-   apply(simp)
-   apply(fastforce)
-  apply(case_tac "m_count ls a")
-   apply(simp)
-  apply(simp)
-  done
+  by (auto simp add: m_count_corres0 split: option.splits)
 
 lemma m_count_corres: "count_list ls x = n \<longleftrightarrow> m_count ls x = (if n=0 then None else Some (n-1))"
   by (simp add: m_count_corres2)
+
 
 text \<open>
 1-(b) Prove that @{term "m_count ls x = None"} is equivalent to
  @{term x} not being a member of @{term ls}.
 \<close>
-find_theorems "count_list"
+
 lemma m_notin: "m_count ls x = None \<longleftrightarrow> x \<notin> set ls"
   by (simp add: m_count_corres2 count_list_0_iff)
 
@@ -111,34 +97,34 @@ text \<open>
  @{term "le (m_count my_ls1) (m_count my_ls2)"} holds.
  Then show that @{term le} is defined correctly by proving it.
 \<close>
+
 (* replace the two undefined below with your multisets *)
 definition "my_ls1 = []"
 definition "my_ls2 = []"
 
 lemma le_example: "le (m_count my_ls1) (m_count my_ls2)"
-  unfolding le_def my_ls1_def my_ls2_def
+  apply(unfold le_def my_ls1_def my_ls2_def)
   by simp
 
 
 text \<open>
 1-(d) Prove that adding an element to a list by @{term Cons} always gives a list
-  greater than the original list.\<close>
+  greater than the original list.
+\<close>
 
 lemma le_m_count: "le (m_count ls) (m_count (x#ls))"
-  apply(unfold le_def)
-  apply(simp split: option.splits)
-  done
+  unfolding le_def
+  by (simp split: option.splits)
 
 
 text \<open>
 1-(e) Prove that @{term m_count} is preserved
   by changing the order of the elements in the list.
 \<close>
+
 lemma m_count_switch:
   "m_count (x # a # ys) = m_count (a # x # ys)"
-  apply(rule ext)
-  apply(simp split: option.split)
-  done
+  by (auto split: option.splits)
 
 lemma m_count_perm:
   "ls = xs @ x # ys  \<Longrightarrow> m_count ls = m_count (x # xs @ ys)"
@@ -157,6 +143,7 @@ next
 qed
 
 
+
 subsection "1.3 Addition of multisets"
 
 text \<open>Next, we consider addition of two multisets. For lists as multisets,
@@ -171,44 +158,41 @@ definition m_add :: "('a, nat) map \<Rightarrow> ('a, nat) map \<Rightarrow> ('a
           | (Some a, None) \<Rightarrow> m1 x
           | (None, _) \<Rightarrow> m2 x"
 
+
 text \<open>
 1-(f) Prove that the empty map is an identity for addition of maps
  (both for left and right).
 \<close>
 
 lemma m_add_empty[simp]: "m_add Map.empty m = m"
-  apply(auto simp: m_add_def)
-  done
+  by (simp add: ext m_add_def)
 
 lemma m_add_empty2[simp]: "m_add m Map.empty = m"
-  apply(rule ext)
-  apply(case_tac "m x")
-   apply(simp add: m_add_def)
-  apply(simp add: m_add_def)
-  done
+  by (simp add: ext m_add_def split: option.splits)
 
 
 text \<open>
-1-(g) Prove that @{term m_add} correctly returns the multiplicity of 
+1-(g) Prove that @{term m_add} correctly returns the multiplicity of
 added multisets, i.e., two lists appended by Isabelle @{term append}.
 \<close>
 
-lemma m_count_x_not_a: "a \<noteq> x \<Longrightarrow> m_count (a # ls) x = m_count ls x"
+lemma m_count_x_not_a:
+  "a \<noteq> x \<Longrightarrow> m_count (a # ls) x = m_count ls x"
   by (simp split: option.splits)
 
-lemma m_count_x_eq_a: "m_count ls x = None \<Longrightarrow> m_count (x # ls) x = Some 0 \<and>
-                       m_count ls x = Some k \<Longrightarrow> m_count (x # ls) x = Some (k+1)"
+lemma m_count_x_eq_a:
+  "m_count ls x = None \<Longrightarrow> m_count (x # ls) x = Some 0 \<and>
+   m_count ls x = Some k \<Longrightarrow> m_count (x # ls) x = Some (k+1)"
   by simp
 
-(* massaging these trivialities into an Isabelle proof made me question my beliefs *)
-(* I guess it's possible to use the correspondence to count_list but... also annoying *)
+(* original 2 page proof preserved for amusement *)
 lemma m_add_append: "m_add (m_count ls1) (m_count ls2) = m_count (append ls1 ls2)"
   apply(induct ls1)
    apply(simp)
   apply(simp only: List.append.append_Cons)
   apply(rule ext)
   apply(case_tac "a\<noteq>x")
-   apply(subgoal_tac "m_add (m_count ls1) (m_count ls2) x 
+   apply(subgoal_tac "m_add (m_count ls1) (m_count ls2) x
                     = m_count (ls1 @ ls2) x")
     apply(insert m_count_x_not_a)[1]
     apply(drule_tac x=a in meta_spec)
@@ -252,7 +236,6 @@ lemma m_add_append: "m_add (m_count ls1) (m_count ls2) = m_count (append ls1 ls2
   done
 
 
-
 subsection "1.4 Sorting of multisets"
 
 text \<open>
@@ -266,18 +249,19 @@ primrec insort' :: "'a::ord \<Rightarrow> 'a list \<Rightarrow> 'a list" where
 
 definition sort' :: "('a::ord) list \<Rightarrow> 'a list" where
   "sort' xs = foldr insort' xs []"
-find_theorems "foldr"
+
 
 text \<open>
 1-(h) With respect to the above sorting function, prove that the sorting of a list
 does not change the multiset it represents; in other words, that @{term sort'}
 preserves multiplicity.
 \<close>
+
 lemma m_count_consg:
   "m_count xs = m_count ys \<Longrightarrow> m_count (b#xs) = m_count (b#ys)"
   by (simp add: m_count_def)
 
-lemma "m_count_insort":
+lemma m_count_insort:
   "m_count (insort' a ys) = m_count (a#ys)"
   apply(induct ys)
    apply(simp)
@@ -292,17 +276,10 @@ lemma "m_count_insort":
 
 lemma m_count_sort_a:
   "m_count (sort' (a # ls)) = m_count (a # sort' ls)"
-  apply(unfold sort'_def)
-  apply(simp)
-  apply(cases "(foldr insort' ls [])")
-   apply(simp)
-  apply(rename_tac y ys)
-  apply(simp only:)
-  apply(case_tac "a \<le> y")
-   apply(simp)
-  apply(simp only: m_count_insort)
-  apply(simp)
-  done
+  unfolding sort'_def
+  apply(simp only: foldr.simps insort'.simps)
+  apply(simp only: Fun.o_apply)
+  by (rule m_count_insort)
 
 lemma m_count_sort':
   "m_count (sort' ls) = m_count ls"
@@ -310,7 +287,7 @@ lemma m_count_sort':
    apply(simp add: sort'_def)
   apply(subgoal_tac " m_count (sort' (a # ls)) = m_count (a # sort' ls)")
    apply(erule trans)
-  apply(erule m_count_consg)
+   apply(erule m_count_consg)
   apply(rule m_count_sort_a)
   done
 
@@ -331,6 +308,7 @@ definition m_union :: "('a, nat) map \<Rightarrow> ('a, nat) map \<Rightarrow> (
 text \<open>
 The union @{text m_Un} of two lists as multisets can be defined as follows:
 \<close>
+
 primrec m_Un' :: "'a list \<Rightarrow> 'a list \<Rightarrow> 'a list \<Rightarrow> 'a list" where
   "m_Un' [] ys ac = ys @ ac"
 | "m_Un' (x#xs) ys ac =
@@ -338,24 +316,16 @@ primrec m_Un' :: "'a list \<Rightarrow> 'a list \<Rightarrow> 'a list \<Rightarr
       else m_Un' xs ys (x#ac))"
 
 definition m_Un where "m_Un l1 l2 = m_Un' l1 l2 []"
-declare [[simp]] m_Un_def
 
 text \<open>
 1-(i) Prove the following lemma about @{term m_Un'} and @{term append}.
 \<close>
+
 lemma ac_append:
   "m_Un' l1 l2 (ac @ ls) = (m_Un' l1 l2 ac) @ ls"
   apply(induct l1 arbitrary: l2 ac)
-   apply(simp)
-  apply(simp)
-  apply(safe)
-   apply(drule_tac x="(remove1 a l2)" in meta_spec)
-   apply(drule_tac x="a#ac" in meta_spec)
-   apply(simp)
-  apply(drule_tac x="l2" in meta_spec)
-  apply(drule_tac x="a#ac" in meta_spec)
-  apply(simp)
-  done
+   apply(simp_all)
+  by (metis append_Cons)
 
 text \<open>
 1-(j) Prove the following lemma about @{term remove1} and @{term m_count}.
@@ -364,29 +334,12 @@ text \<open>
 lemma count_list_remove1:
   "count_list ls a = Suc n \<Longrightarrow> count_list (remove1 a ls) a = n"
   apply(induct ls)
-   apply(simp)
-  apply(auto)
-  done
+  by auto
 
 lemma m_count_remove1_idem:
   "x \<noteq> a \<Longrightarrow> m_count (remove1 a ls) x = m_count ls x"
   apply(induct ls arbitrary: x)
-   apply(simp)
-  apply(case_tac "aa=x")
-   apply(clarsimp)
-  apply(case_tac "m_count ls x")
-    apply(simp)
-   apply(simp)
-  apply(clarsimp)
-  apply(rule conjI)
-   apply(case_tac "m_count ls aa")
-    apply(simp)
-   apply(simp)
-  apply(case_tac "m_count ls aa")
-   apply(simp)
-  apply(drule_tac x=x in meta_spec)
-  apply(simp)
-  done
+  by (auto split: option.splits)
 
 lemma m_count_remove1:
   "m_count (remove1 a ls) =
@@ -405,38 +358,31 @@ lemma m_count_remove1:
      apply(simp add: m_count_corres)
     apply(simp add: m_count_corres2 count_list_remove1)
    apply(simp)
-   apply(thin_tac "m_count ls a = Some 0")
-   apply(simp add: m_count_remove1_idem)
+   apply(erule m_count_remove1_idem)
   apply(rule ext)
   apply(case_tac "x\<noteq>a")
    apply(simp add: m_count_remove1_idem)
-  apply(clarsimp)
   apply(simp add: m_count_corres2 count_list_remove1)
   done
 
 text \<open>
 1-(k) Prove the correctness of @{term m_Un} with respect to @{term m_union}.
 \<close>
+
 lemma count_list_remove1_inv:
   "a \<in> set ls \<Longrightarrow> count_list (remove1 a ls) a = n \<Longrightarrow> count_list ls a = Suc n"
   apply(induct ls)
-   apply(simp)
-  apply(auto)
-  done
+  by auto
 
 lemma count_list_remove1_one:
   "count_list (remove1 a ls) a = 0 \<Longrightarrow> count_list ls a = 1 \<or> count_list ls a = 0"
   apply(induct ls)
-   apply(simp)
-  apply(auto)
-  done
+  by auto
 
 lemma count_list_remove_other:
   "a\<noteq>x \<Longrightarrow> count_list (remove1 a ls) x = count_list ls x"
   apply(induct ls)
-   apply(simp)
-  apply(auto)
-  done
+  by auto
 
 lemma m_un_add: "count_list l1 x = a \<Longrightarrow> count_list l2 x = b \<Longrightarrow> count_list l3 x = c
              \<Longrightarrow> count_list (m_Un' l1 l2 l3) x = c + max a b"
@@ -453,8 +399,8 @@ lemma m_un_add: "count_list l1 x = a \<Longrightarrow> count_list l2 x = b \<Lon
   apply(simp add: count_list_remove_other)
   done
 
-(* wow this one is nice. isomorphism to use existing list theorems :D I see! *)
-lemma m_count_union: "m_count (m_Un l1 l2) = m_union (m_count l1) (m_count l2)"
+lemma m_count_union:
+  "m_count (m_Un l1 l2) = m_union (m_count l1) (m_count l2)"
   unfolding m_union_def
   apply(rule ext)
   apply(case_tac "m_count l1 x")
@@ -520,6 +466,7 @@ where
 
 
 (* ---------- *)
+
 text\<open>
 2-(a): Give an example of an arithmetic expression which evaluates to 7 and uses @{term Plus}
     twice or more. Prove that your example actually evaluates to 7.
@@ -527,22 +474,23 @@ text\<open>
 
 value "(Plus (N 2) (Plus (N 1) (N 4)))"
 lemma "eval (Plus (N 2) (Plus (N 1) (N 4))) (\<lambda>x. 0) = 7"
-  apply(simp)
-  done
+  by simp
+
 
 text\<open>
 2-(b): Prove that the compiler always returns a register identifier strictly higher
   than the one given to it.
 \<close>
+
 lemma compile_reg_increase:
   "compile e r = (p, r') \<Longrightarrow> r' > r"
   apply(induct e arbitrary: p r' r)
-    apply(auto)
-  apply(auto split: prod.splits)
+    apply(auto split: prod.splits)
   apply(fastforce)
   done
 
 (* ---------- *)
+
 subsection "2.1 Target machine big-step semantics and compiler correctness"
 
 (* Big step operational semantics to programs for the register machine *)
@@ -555,7 +503,9 @@ inductive sem :: "mstate \<Rightarrow> rstate \<Rightarrow> bool"
 | sem_Load: "(rs, \<sigma>, Load r v) \<Down> rs(r := \<sigma> v)"
 | sem_Add: "(rs, \<sigma>, Add r1 r2) \<Down> rs(r1 := rs r1 + rs r2)"
 | sem_Seq: "\<lbrakk>(rs, \<sigma>, p) \<Down> rs'; (rs', \<sigma>, q) \<Down> rs''\<rbrakk> \<Longrightarrow> (rs, \<sigma>, p ;; q) \<Down> rs''"
+
 (* ---------- *)
+
 
 text\<open>
 2-(c): Prove that the register machine semantics is deterministic.
@@ -581,22 +531,38 @@ text\<open>
   of identifier lower than the register identifier given to it.
 \<close>
 
+lemma loadI_eval:
+  "(rs, \<sigma>, LoadI r x) \<Down> rs' \<Longrightarrow> rs' = rs(r := x)"
+  by (simp add: sem_LoadI sem_det)
+
+lemma load_eval:
+  "(rs, \<sigma>, Load r v) \<Down> rs' \<Longrightarrow> rs' = rs(r := \<sigma> v)"
+  by (simp add: sem_Load sem_det)
+
 lemma compile_no_modify_lower_reg:
   "compile e r = (p, r') \<Longrightarrow>
    (rs, \<sigma>, p) \<Down> rs' \<Longrightarrow>
    r'' < r \<Longrightarrow>
    rs' r'' = rs r''"
-  thm compile_reg_increase
   apply(induct e arbitrary: r r' r'' rs rs' p)
     apply(clarsimp)
-    (* loadI evaluates to rs[r=x], equal rs' by sem_det, r'' < r *)
-    apply (metis fun_upd_other nat_neq_iff sem_LoadI sem_det)
+    apply(drule loadI_eval, simp)
    apply(clarsimp)
-   apply (metis fun_upd_other nat_neq_iff sem_Load sem_det)
+   apply(drule load_eval, simp)
   apply(simp split: prod.splits)
-  by (smt (verit) compile_reg_increase sem_Add sem_det
-      fun_upd_other nat_neq_iff order_less_trans prod.inject sem.simps
-      prog.distinct(11) prog.distinct(15) prog.distinct(5) prog.inject(4))
+  apply(clarify)
+  apply(erule sem.cases, simp_all)
+  apply(clarify)
+  apply(erule_tac ?a2.0=rs'' in sem.cases, simp_all)
+  apply(clarify)
+  apply(subgoal_tac "rs''a = rs'b(r := rs'b r + rs'b x2)")
+   apply(clarsimp)
+   apply(frule compile_reg_increase)
+   apply(metis order.strict_trans) (* r'' < r < x2 *)
+  apply(erule sem_det)
+  apply(rule sem_Add)
+  done
+
 
 text\<open>
 2-(e): Prove that the compiler produces programs that, when executed, yield the value
@@ -609,15 +575,20 @@ lemma compile_correct:
    (rs, \<sigma>, p) \<Down> rs' \<Longrightarrow>
    rs' r = eval e \<sigma>"
   apply(induct e arbitrary: r r' rs rs' p)
-  apply(simp)
-    apply (metis fun_upd_same sem_LoadI sem_det)
-  apply(simp)
-   apply (metis fun_upd_same sem_Load sem_det)
-  apply(simp split: prod.splits)
-  by (smt (verit) compile_no_modify_lower_reg compile_reg_increase 
-      sem_Add sem_det
-      fst_conv snd_conv fun_upd_same sem.simps
-      prog.distinct(11) prog.distinct(15) prog.distinct(5) prog.inject(4))
+    apply(simp_all split: prod.splits)
+    apply(drule loadI_eval, simp)
+   apply(drule load_eval, simp)
+  apply(erule sem.cases, simp_all)
+  apply(erule_tac ?a2.0=rs'' in sem.cases, simp_all)
+  apply(subgoal_tac "rs''a = rs'b(r := rs'b r + rs'b x2)")
+   apply(frule compile_reg_increase)
+   apply(frule compile_reg_increase)
+   apply(clarsimp)
+   apply(erule_tac rs'=rs'b and p=x1a in compile_no_modify_lower_reg)
+    apply(auto)
+  apply(erule sem_det)
+  apply(rule sem_Add)
+  done
 
 
 (* ---------- *)
@@ -631,11 +602,12 @@ inductive s_sem :: "mstate \<Rightarrow> mstate \<Rightarrow> bool" ("_ \<leadst
 | "(rs, \<sigma>, Add r1 r2) \<leadsto> (rs(r1 := rs r1 + rs r2), \<sigma>, Skip)"
 | "(rs, \<sigma>, p) \<leadsto> (rs', \<sigma>, p') \<Longrightarrow> (rs, \<sigma>, p ;; q) \<leadsto> (rs', \<sigma>, p' ;; q)"
 | "(rs, \<sigma>, Skip ;; p) \<leadsto> (rs, \<sigma>, p)"
-print_theorems
 
 primrec term_with_n_Suc :: "nat \<Rightarrow> aexp" where
   "term_with_n_Suc 0 = N 0"
 | "term_with_n_Suc (Suc n) = (Plus (term_with_n_Suc n) (N 0))"
+
+
 (* ---------- *)
 
 
@@ -647,73 +619,14 @@ that executes n steps of the small-step semantics.
 primrec s_sem_n :: "nat \<Rightarrow> mstate \<Rightarrow> mstate \<Rightarrow> bool" where
   "s_sem_n 0       a b = (a = b)" |
   "s_sem_n (Suc n) a c = (\<exists>b. (a \<leadsto> b) \<and> s_sem_n n b c)"
-print_theorems
+
 
 text\<open>
 2-(g): Prove that two executions of resp. n and m steps according to
    s_sem_n compose into a single execution of (n+m) steps if their
    resp. final and initial machine state match.
 \<close>
-
-lemma s_sem_n_add:
-  "s_sem_n n ms ms' \<Longrightarrow> s_sem_n m ms' ms'' \<Longrightarrow> s_sem_n (n+m) ms ms''"
-  apply(induct n arbitrary: ms)
-   apply(simp)
-  apply(subgoal_tac "\<lbrakk>\<And>ms. \<lbrakk>s_sem_n n ms ms'; s_sem_n m ms' ms''\<rbrakk>
-              \<Longrightarrow> s_sem_n (n + m) ms ms'';
-       \<exists>b. (ms \<leadsto> b) \<and> s_sem_n n b ms'; s_sem_n m ms' ms''\<rbrakk>
-       \<Longrightarrow> s_sem_n (Suc n + m) ms ms''")
-   apply(simp)
-  apply(erule exE)
-  apply(fastforce)
-  done
-
-
-text\<open>
-2-(h): Prove that if p executes to p' in n steps according to s_sem_n, then
-   p ;; q will execute to p' ;; q in n steps with all other parts of the
-   state being the same as in the original execution.
-\<close>
-lemma s_sem_Seq:
-  "s_sem_n (Suc n) (rs, \<sigma>, p) (rs', \<sigma>, p')
-   \<Longrightarrow> \<exists>bs bp. ((rs, \<sigma>, p) \<leadsto> (bs, \<sigma>, bp)) \<and> s_sem_n n (bs, \<sigma>, bp) (rs', \<sigma>, p')"
-  apply(clarsimp)
-  using s_sem.cases
-  apply(fastforce)
-  done
-
-lemma s_sem_n_Seq:
-  "s_sem_n n (rs, \<sigma>, p) (rs', \<sigma>, p') \<Longrightarrow>
-     s_sem_n n (rs, \<sigma>, p;;q) (rs', \<sigma>, p';;q)"
-  apply(induct n arbitrary: rs p)
-   apply(simp)
-  apply(subgoal_tac "\<And>n rs.
-       \<lbrakk>\<And>rs p. s_sem_n n (rs, \<sigma>, p) (rs', \<sigma>, p') \<Longrightarrow>
-             s_sem_n n (rs, \<sigma>, p ;; q) (rs', \<sigma>, p' ;; q);
-        \<exists>bs bp. ((rs, \<sigma>, p) \<leadsto> (bs, \<sigma>, bp)) \<and> s_sem_n n (bs, \<sigma>, bp) (rs', \<sigma>, p')\<rbrakk>
-       \<Longrightarrow> s_sem_n (Suc n) (rs, \<sigma>, p ;; q)
-            (rs', \<sigma>, p' ;; q)")
-   apply(simp add: s_sem_Seq)
-  apply(clarsimp)
-  apply(thin_tac "\<And>rs p. s_sem_n n (rs, \<sigma>, p) (rs', \<sigma>, p') \<Longrightarrow>
-              s_sem_n n (rs, \<sigma>, p ;; q)
-               (rs', \<sigma>, p' ;; q)")
-  apply(thin_tac "s_sem_n n (a, aa, b) (rs', \<sigma>, p')")
-  apply(thin_tac "(rs, \<sigma>, p) \<leadsto> (a, aa, b)")
-  apply(rule_tac x=bs in exI)
-  apply(rule_tac x=\<sigma> in exI)
-  apply(rule_tac x="bp;;q" in exI)
-  apply(auto)
-  apply(simp add: s_sem.intros)
-  done
-
-
-text\<open>
-2-(i): Prove that if a program executes in the big-step semantics to a 
-   resulting rstate rs', then it executes in the small-step semantics
-   to the same resulting rstate and the resulting program Skip with
-   no changes to the vstate.
-\<close>
+(* unused
 lemma s_sem_det:
   "(rs, \<sigma>, p) \<leadsto> b \<Longrightarrow> (rs, \<sigma>, p) \<leadsto> c \<Longrightarrow> b = c"
   apply(induct p arbitrary: rs b c)
@@ -726,24 +639,67 @@ lemma s_sem_det:
    apply(erule s_sem.cases, simp_all)
     apply(erule s_sem.cases, simp_all)
      apply(fastforce)
-    apply(erule s_sem.cases, simp_all)
-   apply(erule s_sem.cases, simp_all)
-   apply(erule s_sem.cases, simp_all)
-  apply(erule s_sem.cases, simp_all)
+    apply(erule s_sem.cases, simp_all)+
   done
+*)
+lemma s_sem_n_add:
+  "s_sem_n n ms ms' \<Longrightarrow> s_sem_n m ms' ms'' \<Longrightarrow> s_sem_n (n+m) ms ms''"
+  apply(induct n arbitrary: ms)
+  apply(simp)
+  by fastforce
+
+
+text\<open>
+2-(h): Prove that if p executes to p' in n steps according to s_sem_n, then
+   p ;; q will execute to p' ;; q in n steps with all other parts of the
+   state being the same as in the original execution.
+\<close>
+
+lemma s_sem_Seq:
+  "s_sem_n (Suc n) (rs, \<sigma>, p) (rs', \<sigma>, p')
+   \<Longrightarrow> \<exists>bs bp. ((rs, \<sigma>, p) \<leadsto> (bs, \<sigma>, bp)) \<and>
+               s_sem_n n (bs, \<sigma>, bp) (rs', \<sigma>, p')"
+  using s_sem.cases
+  by fastforce
+
+lemma s_sem_n_Seq:
+  "s_sem_n n (rs, \<sigma>, p) (rs', \<sigma>, p') \<Longrightarrow>
+     s_sem_n n (rs, \<sigma>, p;;q) (rs', \<sigma>, p';;q)"
+  apply(induct n arbitrary: rs p)
+   apply(simp)
+  apply(subgoal_tac "\<And>n rs.
+       \<lbrakk>\<And>rs p. s_sem_n n (rs, \<sigma>, p) (rs', \<sigma>, p') \<Longrightarrow>
+               s_sem_n n (rs, \<sigma>, p ;; q) (rs', \<sigma>, p' ;; q);
+        \<exists>bs bp. ((rs, \<sigma>, p) \<leadsto> (bs, \<sigma>, bp)) \<and>
+                s_sem_n n (bs, \<sigma>, bp) (rs', \<sigma>, p')\<rbrakk>
+       \<Longrightarrow> s_sem_n (Suc n) (rs, \<sigma>, p ;; q) (rs', \<sigma>, p' ;; q)")
+   apply(simp add: s_sem_Seq)
+  apply(clarsimp)
+  apply(metis s_sem.intros(4))
+  done
+
+
+text\<open>
+2-(i): Prove that if a program executes in the big-step semantics to a
+   resulting rstate rs', then it executes in the small-step semantics
+   to the same resulting rstate and the resulting program Skip with
+   no changes to the vstate.
+\<close>
 
 lemma s_sem_n_correct:
   "ms \<Down> rs' \<Longrightarrow> \<exists>n. s_sem_n n ms (rs', fst (snd ms), Skip)"
-  apply(erule sem.induct)
+  apply(induct ms rs' rule: sem.induct)
      apply(simp_all del: Fun.fun_upd_apply)
      apply(rule exI[where x=1])
      apply(simp del: Fun.fun_upd_apply)
      apply(rule_tac s_sem.intros(1))
-    apply(metis s_sem.intros s_sem_n.simps)
-   apply(metis s_sem.intros s_sem_n.simps)
+    apply(metis s_sem.intros(2) s_sem_n.simps) (* etc *)
+   apply(metis s_sem.intros(3) s_sem_n.simps)
   apply(clarsimp)
-  apply(meson s_sem.intros s_sem_n.simps s_sem_n_Seq s_sem_n_add)
-  done
+  apply(drule_tac q=q in s_sem_n_Seq)
+  apply(cut_tac rs=rs' and p=q and \<sigma>=\<sigma> in s_sem.intros(5))
+  using s_sem_n.simps(2) s_sem_n_add
+  by fastforce
 
 
 text\<open>
@@ -754,9 +710,7 @@ text\<open>
 lemma compile_term_with_n_Suc_lower_bound_n:
    "h < snd (compile (term_with_n_Suc h) r) - r"
   apply(induct h)
-   apply(simp)
-  apply(auto split: prod.splits)
-  done
+  by (auto split: prod.splits)
 
 
 text\<open>
@@ -771,7 +725,6 @@ lemma compile_has_no_universal_register_bound:
   apply(cut_tac h=h and r=r in compile_term_with_n_Suc_lower_bound_n)
   apply(fastforce)
   done
-
 
 (*---------------------------------------------------------*)
 
